AwsCryptographicMaterialProviders/dafny/AwsCryptographyKeyStore/test/Fixtures.dfy
@@ -6,8 +6,13 @@ include "../src/Index.dfy"
 module Fixtures {
   import opened StandardLibrary.UInt
   import Types = AwsCryptographyKeyStoreTypes
+  import DDB = Com.Amazonaws.Dynamodb
+  import KMS = Com.Amazonaws.Kms
   import UTF8
+  import Seq
   import opened Wrappers
+  import KeyStore
+  import Structure
 
   method EncodeEncryptionContext(
     input: map<string,string>
@@ -51,6 +56,9 @@ module Fixtures {
     output := Success(map i <- decodedEncryptionContext :: i.0.value := i.1.value);
   }
 
+  // Python method for getting Dafny byte sequence
+  // def as_dafny_bytes(string):
+  //   return "[" +  ", ".join(["0x" + character.encode("utf-8").hex() for character in string]) + "]"
   const abc : UTF8.ValidUTF8Bytes :=
     var s := [0x61, 0x62, 0x63];
     assert s == UTF8.EncodeAscii("abc");
@@ -62,12 +70,16 @@ module Fixtures {
     s
 
   // The following are test resources that exist in tests accounts:
-
   const branchKeyStoreName := "KeyStoreDdbTable"
   const logicalKeyStoreName := branchKeyStoreName
+  // Static Key Store Names (This uses the same logical key store name as in branchKeyStoreName)
+  const staticBranchKeyStoreName := "KeyStoreStaticTable"
+  const staticLogicalKeyStoreName := branchKeyStoreName
+  // hierarchy-version-1 branch key
   const branchKeyId := "3f43a9af-08c5-4317-b694-3d3e883dcaef"
   const branchKeyIdActiveVersion := "a4905627-4b7f-4272-a847-f50dae245737"
   // This is branchKeyIdActiveVersion above, as utf8bytes
+  // https://cyberchef.infosec.amazon.dev/#recipe=Encode_text('UTF-8%20(65001)')To_Decimal('Comma',false)&input=YTQ5MDU2MjctNGI3Zi00MjcyLWE4NDctZjUwZGFlMjQ1NzM3&oenc=65001
   const branchKeyIdActiveVersionUtf8Bytes: seq<uint8> := [
     97, 52, 57, 48, 53, 54, 50, 55, 45, 52,
     98, 55, 102, 45, 52, 50, 55, 50, 45, 97,
@@ -75,13 +87,26 @@ module Fixtures {
     50, 52, 53, 55, 51, 55
   ]
   const branchKeyIdWithEC := "4bb57643-07c1-419e-92ad-0df0df149d7c"
-
+  // hierarchy-version-2 branch key
+  const hv2BranchKeyId := "4a0c7b92-3703-4209-8961-24b07ab6562b"
+  const hv2BranchKeyVersion := "a0496b5c-e048-42bc-8b75-68a004851803"
+  // This is hv2BranchKeyVersion above, as utf8bytes
+  // https://cyberchef.infosec.amazon.dev/#recipe=Encode_text('UTF-8%20(65001)')To_Decimal('Comma',false)&input=YTA0OTZiNWMtZTA0OC00MmJjLThiNzUtNjhhMDA0ODUxODAz&oenc=65001
+  const hv2BranchKeyIdActiveVersionUtf8Bytes: seq<uint8> := [
+    97, 48, 52, 57, 54, 98, 53, 99, 45, 101, 48, 52,
+    56, 45, 52, 50, 98, 99, 45, 56, 98, 55, 53, 45,
+    54, 56, 97, 48, 48, 52, 56, 53, 49, 56, 48, 51
+  ]
   // THESE ARE TESTING RESOURCES DO NOT USE IN A PRODUCTION ENVIRONMENT
   const keyArn := "arn:aws:kms:us-west-2:370957321024:key/9d989aa2-2f9c-438c-a745-cc57d3ad0126"
+  const kmsArnForHV1 := "arn:aws:kms:us-west-2:370957321024:key/85cee5a8-fecb-41e9-affd-a1f7bb036884"
+  const kmsArnForHV2 := "arn:aws:kms:us-west-2:370957321024:key/da179005-1c04-4b91-a103-ee43b9a707e6"
   const keyId := "9d989aa2-2f9c-438c-a745-cc57d3ad0126"
 
   // mrkRsaKeyArn is an RSA Key
   const mrkRsaKeyArn := "arn:aws:kms:us-west-2:370957321024:key/mrk-63d386cb70614ea59b32ad65c9315297"
+  const lyingBranchKeyId := "kms-arn-attribute-is-lying"
+  const lyingBranchKeyDecryptOnlyVersion := "129c5c87-308a-41c9-8b9d-a27f66e915f4"
 
   const MrkArnEast : string := "arn:aws:kms:us-east-1:658956600833:key/mrk-80bd8ecdcd4342aebd84b7dc9da498a7"
   const MrkArnWest : string := "arn:aws:kms:us-west-2:658956600833:key/mrk-80bd8ecdcd4342aebd84b7dc9da498a7"
@@ -95,9 +120,25 @@ module Fixtures {
   const KmsSrkConfigWest : Types.KMSConfiguration := Types.KMSConfiguration.kmsKeyArn(MrkArnWest)
   const KmsMrkConfigAP : Types.KMSConfiguration := Types.KMSConfiguration.kmsMRKeyArn(MrkArnAP)
   const KmsMrkEC : Types.EncryptionContext := map[abc := x123]
+  const RobbieEC : Types.EncryptionContext := map[Robbie := IsADog]
+  const RobbieECString : Structure.EncryptionContextString := map["Robbie" := "Is a dog."]
+  const KodaECString : Structure.EncryptionContextString := map["Koda" := "Is a dog."]
   const EastBranchKey : string := "MyEastBranch2"
+  const EastBranchKeyIdActiveVersion : string := "6f22825b-bd56-4434-83e2-2782e2160172"
+  const EastBranchKeyBranchKeyIdActiveVersionUtf8Bytes: seq<uint8> := [
+    54, 102, 50, 50, 56, 50, 53, 98, 45, 98, 100,
+    53, 54, 45, 52, 52, 51, 52, 45, 56, 51, 101, 50,
+    45, 50, 55, 56, 50, 101, 50, 49, 54, 48, 49, 55, 50
+  ]
   const WestBranchKey : string := "MyWestBranch2"
+  const WestBranchKeyIdActiveVersion : string := "094715a4-b98d-4c98-bf50-17422a8938f4"
+  const WestBranchKeyBranchKeyIdActiveVersionUtf8Bytes: seq<uint8> := [
+    48, 57, 52, 55, 49, 53, 97, 52, 45, 98, 57, 56,
+    100, 45, 52, 99, 57, 56, 45, 98, 102, 53, 48, 45,
+    49, 55, 52, 50, 50, 97, 56, 57, 51, 56, 102, 52
+  ]
   const publicKeyArn := "arn:aws:kms:us-west-2:658956600833:key/b3537ef1-d8dc-4780-9f5a-55776cbb2f7f"
+  const kmsSystemKey := "arn:aws:kms:us-west-2:370957321024:key/6613e250-b2e7-4c4c-a54e-2b241f837242"
 
   // TODO: After ~2024/06/11 launch, add the next two lines to cfn/ESDK-Hierarchy-CI.yaml
   const postalHornKeyArn := "arn:aws:kms:us-west-2:370957321024:key/bc127593-f7da-452c-a1f3-cd34c46f81f8"
@@ -107,6 +148,472 @@ module Fixtures {
 
   // Creation of this particular illegal Branch Key is detailed here:
   // `git rev-parse --show-toplevel`/cfn/lyingBranchKeyCreation.md
-  const lyingBranchKeyId := "kms-arn-attribute-is-lying"
-  const lyingBranchKeyDecryptOnlyVersion := "129c5c87-308a-41c9-8b9d-a27f66e915f4"
+  const hierarchyV1InvalidKmsArnId := "kms-arn-attribute-is-lying"
+  const hierarchyV1InvalidKmsArnVersion := "129c5c87-308a-41c9-8b9d-a27f66e915f4"
+  // TODO-HV-2-FF : Document creation of lying branch keys
+  const hierarchyV2InvalidKmsArnId := "DO-NOT-DELETE-test-hv2-get-key-wrong-kms-arn"
+  const hierarchyV2InvalidKmsArnVersion := "e3df6cf8-3edc-4781-998e-c4731b755452"
+
+  const hierarchyV2InvalidDigestId := "DO-NOT-DELETE-test-hv2-get-key-wrong-digest"
+  const hierarchyV2InvalidDigestVersion := "755404a1-a295-4ec9-ba13-c540e16515d5"
+
+  const hierarchyV2InvalidCiphertextId := "DO-NOT-DELETE-test-hv2-get-key-wrong-ciphertext"
+  const hierarchyV2InvalidCiphertextVersion := "94a3bb88-bbaa-4830-99d4-7a949a02f4a1"
+
+  const hierarchyV2InvalidPlaintextLengthId := "DO-NOT-DELETE-test-hv2-get-key-wrong-ciphertext-length"
+  const hierarchyV2InvalidPlaintextLengthVersion := "04b459a3-0731-4ba8-b9ac-4e29eb6db485"
+
+  const hierarchyV2MissingPrefixedECId := "DO-NOT-DELETE-test-hv2-get-key-missing-prefixed-ec"
+  const hierarchyV2MissingPrefixedECVersion := "d3e7b039-71fb-41af-8549-2564a170935c"
+
+  const hierarchyV2UnexpectedECId := "DO-NOT-DELETE-test-hv2-get-key-unexpected-ec"
+  const hierarchyV2UnexpectedECVersion := "a01eec17-9b1c-4f4a-9b66-2c84816854ac"
+
+  // Constants for Testing Storage
+  const ORIGINAL_BYTES : UTF8.ValidUTF8Bytes :=
+    var s := [0x73, 0x74, 0x6f, 0x72, 0x61, 0x67, 0x65, 0x2d, 0x64, 0x6f, 0x65, 0x73, 0x2d, 0x6e, 0x6f, 0x74, 0x2d, 0x76, 0x61, 0x6c, 0x69, 0x64, 0x61, 0x74, 0x65, 0x2d, 0x6f, 0x72, 0x69, 0x67, 0x69, 0x6e, 0x61, 0x6c, 0x2d, 0x6f, 0x6e, 0x6c, 0x79, 0x2d, 0x74, 0x68, 0x61, 0x74, 0x2d, 0x69, 0x73, 0x2d, 0x62, 0x69, 0x6e, 0x61, 0x72, 0x79];
+    assert s == UTF8.EncodeAscii("storage-does-not-validate-original-only-that-is-binary");
+    s
+
+  const TERMINAL_BYTES : UTF8.ValidUTF8Bytes :=
+    var s := [0x73, 0x74, 0x6f, 0x72, 0x61, 0x67, 0x65, 0x2d, 0x64, 0x6f, 0x65, 0x73, 0x2d, 0x6e, 0x6f, 0x74, 0x2d, 0x76, 0x61, 0x6c, 0x69, 0x64, 0x61, 0x74, 0x65, 0x2d, 0x74, 0x65, 0x72, 0x6d, 0x69, 0x6e, 0x61, 0x6c, 0x2d, 0x6f, 0x6e, 0x6c, 0x79, 0x2d, 0x74, 0x68, 0x61, 0x74, 0x2d, 0x69, 0x73, 0x2d, 0x62, 0x69, 0x6e, 0x61, 0x72, 0x79];
+    assert s == UTF8.EncodeAscii("storage-does-not-validate-terminal-only-that-is-binary");
+    s
+
+  const INPUT_BYTES : UTF8.ValidUTF8Bytes :=
+    var s := [0x73, 0x74, 0x6f, 0x72, 0x61, 0x67, 0x65, 0x2d, 0x64, 0x6f, 0x65, 0x73, 0x2d, 0x6e, 0x6f, 0x74, 0x2d, 0x76, 0x61, 0x6c, 0x69, 0x64, 0x61, 0x74, 0x65, 0x2d, 0x69, 0x6e, 0x70, 0x75, 0x74, 0x2d, 0x6f, 0x6e, 0x6c, 0x79, 0x2d, 0x74, 0x68, 0x61, 0x74, 0x2d, 0x69, 0x73, 0x2d, 0x62, 0x69, 0x6e, 0x61, 0x72, 0x79];
+    assert s == UTF8.EncodeAscii("storage-does-not-validate-input-only-that-is-binary");
+    s
+
+  const ENC_BYTES : UTF8.ValidUTF8Bytes :=
+    var s := [0x73, 0x74, 0x6f, 0x72, 0x61, 0x67, 0x65, 0x2d, 0x64, 0x6f, 0x65, 0x73, 0x2d, 0x6e, 0x6f, 0x74, 0x2d, 0x76, 0x61, 0x6c, 0x69, 0x64, 0x61, 0x74, 0x65, 0x2d, 0x65, 0x6e, 0x63, 0x2d, 0x6f, 0x6e, 0x6c, 0x79, 0x2d, 0x74, 0x68, 0x61, 0x74, 0x2d, 0x69, 0x73, 0x2d, 0x62, 0x69, 0x6e, 0x61, 0x72, 0x79];
+    assert s == UTF8.EncodeAscii("storage-does-not-validate-enc-only-that-is-binary");
+    s
+
+  const NOW_BYTES : UTF8.ValidUTF8Bytes :=
+    var s := [0x6e, 0x6f, 0x77];
+    assert s == UTF8.EncodeAscii("now");
+    s
+
+  // This function is the lie we will tell ourselves
+  // about what the mutation scope is.
+  // You MUST NOT reveal this value.
+  function {:opaque} FixturesLie(): set<object>
+  {{}}
+
+  method ProvideDDBClient(
+    ddbClient?: Option<DDB.Types.IDynamoDBClient> := None
+  )
+    returns (output: Result<DDB.Types.IDynamoDBClient, DDB.Types.Error>)
+    requires ddbClient?.Some? ==> ddbClient?.value.ValidState()
+    modifies (if ddbClient?.Some? then ddbClient?.value.Modifies else {})
+    ensures output.Success?
+            ==>
+              && output.value.ValidState()
+              && fresh(output.value)
+              && fresh(output.value.Modifies)
+  {
+    var ddbClient: DDB.Types.IDynamoDBClient;
+    if (ddbClient?.None?) {
+      ddbClient :- DDB.DynamoDBClient();
+    } else {
+      ddbClient := ddbClient?.value;
+    }
+    assume {:axiom} ddbClient.Modifies < FixturesLie();
+    assume {:axiom} fresh(ddbClient) && fresh(ddbClient.Modifies);
+    return Success(ddbClient);
+  }
+
+  method ProvideKMSClient(
+    kmsClient?: Option<KMS.Types.IKMSClient> := None
+  )
+    returns (output: Result<KMS.Types.IKMSClient, KMS.Types.Error>)
+    requires kmsClient?.Some? ==> kmsClient?.value.ValidState()
+    modifies (if kmsClient?.Some? then kmsClient?.value.Modifies else {})
+    ensures output.Success?
+            ==>
+              && output.value.ValidState()
+              && fresh(output.value)
+              && fresh(output.value.Modifies)
+  {
+    var kmsClient: KMS.Types.IKMSClient;
+    if (kmsClient?.None?) {
+      kmsClient :- KMS.KMSClient();
+    } else {
+      kmsClient := kmsClient?.value;
+    }
+    assume {:axiom} kmsClient.Modifies < FixturesLie();
+    assume {:axiom} fresh(kmsClient) && fresh(kmsClient.Modifies);
+    return Success(kmsClient);
+  }
+
+  method DefaultKeyStore(
+    nameonly kmsId: string := keyArn,
+    nameonly physicalName: string := branchKeyStoreName,
+    nameonly logicalName: string := logicalKeyStoreName,
+    nameonly ddbClient?: Option<DDB.Types.IDynamoDBClient> := None,
+    nameonly kmsClient?: Option<KMS.Types.IKMSClient> := None
+  )
+    returns (output: Result<Types.IKeyStoreClient, Types.Error>)
+    requires DDB.Types.IsValid_TableName(physicalName)
+    requires KMS.Types.IsValid_KeyIdType(kmsId)
+    requires ddbClient?.Some? ==> ddbClient?.value.ValidState()
+    requires kmsClient?.Some? ==> kmsClient?.value.ValidState()
+    ensures output.Success? ==> output.value.ValidState()
+    modifies (if ddbClient?.Some? then ddbClient?.value.Modifies else {})
+             + (if kmsClient?.Some? then kmsClient?.value.Modifies else {})
+    ensures output.Success?
+            ==>
+              && output.value.ValidState()
+              && fresh(output.value)
+              && fresh(output.value.Modifies)
+  {
+    var ddbClient :- expect ProvideDDBClient(ddbClient?);
+    assume {:axiom} fresh(ddbClient) && fresh(ddbClient.Modifies);
+    var kmsClient :- expect ProvideKMSClient(kmsClient?);
+    assume {:axiom} fresh(kmsClient) && fresh(kmsClient.Modifies);
+    var kmsConfig := Types.KMSConfiguration.kmsKeyArn(kmsId);
+    var keyStoreConfig := Types.KeyStoreConfig(
+      ddbTableName := physicalName,
+      kmsConfiguration := kmsConfig,
+      logicalKeyStoreName := logicalName,
+      id := None,
+      ddbClient := ddbClient?,
+      kmsClient := kmsClient?
+    );
+    var keyStore :- expect KeyStore.KeyStore(keyStoreConfig);
+    assume {:axiom} fresh(keyStore.Modifies);
+    return Success(keyStore);
+  }
+  method StaticKeyStore(
+    nameonly kmsId: string := keyArn,
+    nameonly physicalName: string := staticBranchKeyStoreName,
+    nameonly logicalName: string := staticLogicalKeyStoreName,
+    nameonly ddbClient?: Option<DDB.Types.IDynamoDBClient> := None,
+    nameonly kmsClient?: Option<KMS.Types.IKMSClient> := None
+  )
+    returns (output: Result<Types.IKeyStoreClient, Types.Error>)
+    requires DDB.Types.IsValid_TableName(physicalName)
+    requires KMS.Types.IsValid_KeyIdType(kmsId)
+    requires ddbClient?.Some? ==> ddbClient?.value.ValidState()
+    requires kmsClient?.Some? ==> kmsClient?.value.ValidState()
+    ensures output.Success? ==> output.value.ValidState()
+    modifies (if ddbClient?.Some? then ddbClient?.value.Modifies else {})
+             + (if kmsClient?.Some? then kmsClient?.value.Modifies else {})
+    ensures output.Success?
+            ==>
+              && output.value.ValidState()
+              && fresh(output.value)
+              && fresh(output.value.Modifies)
+  {
+    output := DefaultKeyStore(
+      kmsId := kmsId,
+      physicalName := physicalName,
+      logicalName := logicalName,
+      ddbClient? := ddbClient?,
+      kmsClient? := kmsClient?
+    );
+  }
+
+  method KeyStoreFromKMSConfig(
+    nameonly kmsConfig: Types.KMSConfiguration,
+    nameonly physicalName: string := branchKeyStoreName,
+    nameonly logicalName: string := logicalKeyStoreName,
+    nameonly ddbClient?: Option<DDB.Types.IDynamoDBClient> := None
+  )
+    returns (output: Result<Types.IKeyStoreClient, Types.Error>)
+    requires DDB.Types.IsValid_TableName(physicalName)
+    ensures output.Success? ==> output.value.ValidState()
+    ensures output.Success?
+            ==>
+              && output.value.ValidState()
+              && fresh(output.value)
+              && fresh(output.value.Modifies)
+  {
+    if ddbClient?.Some? {
+      assume {:axiom} fresh(ddbClient?.value) && fresh(ddbClient?.value.Modifies);
+    }
+    var keyStoreConfig := Types.KeyStoreConfig(
+      ddbTableName := physicalName,
+      id := None,
+      kmsConfiguration := kmsConfig,
+      logicalKeyStoreName := logicalName,
+      ddbClient := ddbClient?
+    );
+    var keyStore :- expect KeyStore.KeyStore(keyStoreConfig);
+    return Success(keyStore);
+  }
+  /*
+    nameonly ddbTableName: ComAmazonawsDynamodbTypes.TableName ,
+    nameonly kmsConfiguration: KMSConfiguration ,
+    nameonly logicalKeyStoreName: string ,
+    nameonly id: Option<string> := Option.None ,
+    nameonly grantTokens: Option<GrantTokenList> := Option.None ,
+    nameonly ddbClient: Option<ComAmazonawsDynamodbTypes.IDynamoDBClient> := Option.None ,
+    nameonly kmsClient: Option<ComAmazonawsKmsTypes.IKMSClient> := Option.None
+*/
+
+
+  datatype allThree = | allThree (
+    active: Structure.EncryptedHierarchicalKey,
+    beacon: Structure.EncryptedHierarchicalKey,
+    decrypt: Structure.EncryptedHierarchicalKey)
+  /*
+    method getItems(
+      nameonly id: string,
+      nameonly underTest: Types.IKeyStorageInterface
+    )
+      returns (output: Result<allThree, Types.Error>)
+      requires underTest.ValidState()
+      ensures underTest.ValidState()
+      modifies underTest.Modifies
+    {
+      var activeInput := Types.GetEncryptedActiveBranchKeyInput(
+        Identifier := id
+      );
+      var active? :- underTest.GetEncryptedActiveBranchKey(activeInput);
+      var active := active?.Item;
+  
+      var beaconInput := Types.GetEncryptedBeaconKeyInput(
+        Identifier := id
+      );
+      var beacon? :- underTest.GetEncryptedBeaconKey(beaconInput);
+      var beacon := beacon?.Item;
+  
+      expect active.Type.ActiveHierarchicalSymmetricVersion?;
+      var decryptInput := Types.GetEncryptedBranchKeyVersionInput(
+        Identifier := id,
+        Version := active.Type.ActiveHierarchicalSymmetricVersion.Version
+      );
+      var decrypt? :- underTest.GetEncryptedBranchKeyVersion(decryptInput);
+      var decrypt := decrypt?.Item;
+      output := Success(allThree(active, beacon, decrypt));
+    }
+  */
+  const Robbie : UTF8.ValidUTF8Bytes :=
+    var s := [0x52, 0x6f, 0x62, 0x62, 0x69, 0x65];
+    assert s == UTF8.EncodeAscii("Robbie");
+    s
+
+  const Koda : UTF8.ValidUTF8Bytes :=
+    var s := [0x4b, 0x6f, 0x64, 0x61];
+    assert s == UTF8.EncodeAscii("Koda");
+    s
+
+  const IsADog : UTF8.ValidUTF8Bytes :=
+    var s := [0x49, 0x73, 0x20, 0x61, 0x20, 0x64, 0x6f, 0x67, 0x2e];
+    assert s == UTF8.EncodeAscii("Is a dog.");
+    s
+
+  method CreateHappyCaseId(
+    nameonly id: string,
+    nameonly kmsId: string := keyArn,
+    nameonly physicalName: string := branchKeyStoreName,
+    nameonly logicalName: string := logicalKeyStoreName,
+    nameonly versionCount: nat := 3,
+    nameonly customEC: Types.EncryptionContext := RobbieEC
+  )
+    requires DDB.Types.IsValid_TableName(physicalName)
+    requires KMS.Types.IsValid_KeyIdType(kmsId)
+    requires 0 <= versionCount <= 5
+    requires 0 < |customEC| // requires some EC
+  {
+    var keyStore :- expect DefaultKeyStore(kmsId:=kmsId, physicalName:=physicalName, logicalName:=logicalName);
+    assume {:axiom} fresh(keyStore) && fresh(keyStore.Modifies);
+    var input := Types.CreateKeyInput(
+      branchKeyIdentifier := Some(id),
+      encryptionContext := Some(customEC)
+    );
+    var branchKeyId :- expect keyStore.CreateKey(input);
+
+    // If you need a new version
+    var inputV := Types.VersionKeyInput(
+      branchKeyIdentifier := id
+    );
+    var versionIndex := 0;
+    while versionIndex < versionCount {
+      var _ :- expect keyStore.VersionKey(inputV);
+      versionIndex := versionIndex + 1;
+    }
+  }
+
+  method GetItemFromDDB(
+    nameonly id: string,
+    nameonly typeStr: string,
+    nameonly physicalName: string := branchKeyStoreName,
+    nameonly ddbClient?: Option<DDB.Types.IDynamoDBClient> := None
+  )
+    returns (output: Result<DDB.Types.AttributeMap, string>)
+    requires DDB.Types.IsValid_TableName(physicalName)
+    requires ddbClient?.Some? ==> ddbClient?.value.ValidState()
+    modifies (if ddbClient?.Some? then ddbClient?.value.Modifies else {})
+  {
+    var ddbClient: DDB.Types.IDynamoDBClient;
+    if (ddbClient?.None?) {
+      ddbClient :- expect DDB.DynamoDBClient();
+    } else {
+      ddbClient := ddbClient?.value;
+    }
+    var input := DDB.Types.GetItemInput(
+      TableName := physicalName,
+      Key := map[
+        Structure.BRANCH_KEY_IDENTIFIER_FIELD := DDB.Types.AttributeValue.S(id),
+        Structure.TYPE_FIELD := DDB.Types.AttributeValue.S(typeStr)
+      ],
+      ConsistentRead := Some(true));
+    var result? := ddbClient.GetItem(input);
+    if (result?.Success? && result?.value.Item.Some? && 0 < |result?.value.Item.value| ) {
+      return Success(result?.value.Item.value);
+    }
+    return Failure("Failed to GetItem. ID: " + id + " type: " + typeStr + " .");
+  }
+
+  method CopyBranchKey(
+    nameonly Identifier: string,
+    nameonly sourceTableName: string,
+    nameonly targetTableName: string,
+    nameonly ddbClient: DDB.Types.IDynamoDBClient
+  )
+    returns (output: Result<bool, DDB.Types.Error>)
+    requires
+      && ddbClient.ValidState()
+      && DDB.Types.IsValid_TableName(sourceTableName)
+      && DDB.Types.IsValid_TableName(targetTableName)
+    modifies ddbClient.Modifies
+    ensures ddbClient.ValidState()
+  {
+    // Query to get all items with the specified branch key ID
+    var ExpressionAttributeNames := map[
+      "#pk" := Structure.BRANCH_KEY_IDENTIFIER_FIELD
+    ];
+    var ExpressionAttributeValues := map[
+      ":pk" := DDB.Types.AttributeValue.S(Identifier)
+    ];
+    var queryReq := DDB.Types.QueryInput(
+      TableName := sourceTableName,
+      KeyConditionExpression := Some("#pk = :pk"),
+      ExpressionAttributeNames := Some(ExpressionAttributeNames),
+      ExpressionAttributeValues := Some(ExpressionAttributeValues)
+    );
+
+    // Execute the query
+    var queryRes :- ddbClient.Query(queryReq);
+    if (queryRes.Items.None?) {
+      return Success(true);
+    }
+
+    // Create put requests for each item
+    var putItems: seq<DDB.Types.TransactWriteItem> :- Seq.MapWithResult(
+      (item: DDB.Types.AttributeMap)
+      =>
+        :- Need(
+             Structure.TYPE_FIELD in item,
+             DDB.Types.Error.InternalServerError(message := Some("Item missing required type field"))
+           );
+        Success(
+          DDB.Types.TransactWriteItem(
+            Put := Some(
+              DDB.Types.Put(
+                Item := item,
+                TableName := targetTableName
+              )))),
+      queryRes.Items.value);
+
+    if (0 == |putItems|) {
+      return Success(true);
+    }
+
+    // DynamoDB transactions are limited to 100 items
+    var allItemsCopied := true;
+    var remainingItems := putItems;
+
+    while |remainingItems| > 0
+      decreases |remainingItems|
+    {
+      var batchItems := if |remainingItems| > 100
+      then remainingItems[..100]
+      else remainingItems;
+
+      var writeReq := DDB.Types.TransactWriteItemsInput(
+        TransactItems := batchItems
+      );
+      var _ :- ddbClient.TransactWriteItems(writeReq);
+
+      if |remainingItems| > 100 {
+        remainingItems := remainingItems[100..];
+        allItemsCopied := false;
+      } else {
+        remainingItems := [];
+      }
+    }
+
+    return Success(allItemsCopied);
+  }
+
+  method CopyAllStaticBranchKeys(
+    nameonly ddbClient: DDB.Types.IDynamoDBClient
+  )
+    returns (output: Result<bool, DDB.Types.Error>)
+    requires ddbClient.ValidState()
+    modifies ddbClient.Modifies
+    ensures ddbClient.ValidState()
+  {
+    // List of (branchKeyId, hierarchyVersion)
+    var branchKeys := [
+      // HV1 Branch Keys
+      branchKeyId,
+      branchKeyIdWithEC,
+      hierarchyV1InvalidKmsArnId,
+      EastBranchKey,
+      WestBranchKey,
+      postalHornBranchKeyId,
+      "STATIC-PRE-HV-2-MUTATION-WITH-SYSTEM-KEY",
+      "STATIC-PRE-HV-2-MUTATION-WITH-TRUST-STORAGE",
+
+      // HV2 Branch Keys
+      hv2BranchKeyId,
+      hierarchyV2InvalidKmsArnId,
+      hierarchyV2InvalidDigestId,
+      hierarchyV2InvalidCiphertextId,
+      hierarchyV2InvalidPlaintextLengthId,
+      hierarchyV2MissingPrefixedECId,
+      hierarchyV2UnexpectedECId
+    ];
+
+    var idx := 0;
+    while idx < |branchKeys|
+      decreases |branchKeys| - idx
+    {
+      var id := branchKeys[idx];
+      var _ :- CopyBranchKey(
+        Identifier := id,
+        sourceTableName := branchKeyStoreName,
+        targetTableName := staticBranchKeyStoreName,
+        ddbClient := ddbClient
+      );
+
+      idx := idx + 1;
+    }
+
+    return Success(true);
+  }
+  /*
+    // Test to Copy All Static Branch Keys from `KeyStoreDdbTable` to `KeyStoreStaticTable`
+    //
+    // IMPORTANT:
+    // The CI role does not have write access to `KeyStoreStaticTable` by default.
+    // To copy static branch keys to the static key store table, you must:
+    //   1. Assume the Admin role for the CI account
+    //   2. Run this test with the proper IAM permissions
+    //   3. Verify all keys were copied successfully
+    //
+    // This test should be performed carefully and only when necessary,
+    // such as when setting up test environments or refreshing static test data.
+    method {:test} TestCopyAllBranchKeys()
+    {
+      var ddbClient :- expect ProvideDDBClient();
+      var success :- expect CopyAllStaticBranchKeys(ddbClient := ddbClient);
+      expect success, "Failed to copy all branch keys";
+    }
+  */
 }
